README.md
@@ -4,12 +4,17 @@ Subset of TIP as defined in _Static Program Analysis_. Approach influenced by _P
 
 The goal is to develop complete, end-to-end proofs of dataflow soundness in Lean, establishing correctness of the procedure (fixpoint computation) as well as correctness wrt language semantics.
 
-Progress:
-- [x] Formalized Kildall's worklist algorithm. 
-  - [x] Proof of termination
-  - [x] Proof of soundness
-- [x] Example of "mundane" correctness as described in PPA.
-  - [x] Constant propagation
-- [ ] Collection semantics proven by "mundane" correctness
-- [ ] Galois connections between collection semantics and further analyses.
+Implemented so far : 
 
+- Subset of TIP : syntax and CEK semantics.
+- CFG builder
+- Kildall's Worklist algorithm (verified to be terminating and sound)
+- Generic dataflow framework
+- Decorated semantics over the CEK semantics, proven equivalent to the original
+- Two analyses (Constant Propagation, Collection Semantics)
+- Correctness for the two analyses!
+
+Remains:
+- [ ] Lots Lots Lots of cleanup
+- [ ] Galois connections between collection semantics and further analyses for 
+      more composable proofs.
